theories/typing/cont.v
@@ -9,7 +9,7 @@ Section typing.
 
   (** Jumping to and defining a continuation. *)
   Lemma type_jump E L C T k args T' :
-    CCtx_iscont k L _ T' ∈ C →
+    (k ◁cont(L, T'))%CC ∈ C →
     tctx_incl E L T (T' (list_to_vec args)) →
     typed_body E L C T (k (of_val <$> args)).
   Proof.
@@ -21,9 +21,9 @@ Section typing.
 
   Lemma type_cont E L1 L2 C T argsb econt e2 T' kb :
     Closed (kb :b: argsb +b+ []) econt → Closed (kb :b: []) e2 →
-    (∀ k args, typed_body E L1 (CCtx_iscont k L1 _ T' :: C) (T' args)
+    (∀ k args, typed_body E L1 (k ◁cont(L1, T') :: C) (T' args)
                           (subst_v (kb::argsb) (k:::args) econt)) →
-    (∀ k, typed_body E L2 (CCtx_iscont k L1 _ T' :: C) T (subst' kb k e2)) →
+    (∀ k, typed_body E L2 (k ◁cont(L1, T') :: C) T (subst' kb k e2)) →
     typed_body E L2 C T (let: kb := Rec kb argsb econt in e2).
   Proof.
     iIntros (Hc1 Hc2 Hecont He2 tid qE) "#HEAP #LFT Htl HE HL HC HT". iApply wp_let'.
