theories/typing/shr_bor.v
@@ -55,8 +55,7 @@ Section typing.
 
   Lemma tctx_reborrow_shr E L p ty κ κ' :
     lctx_lft_incl E L κ' κ →
-    tctx_incl E L [TCtx_hasty p (&shr{κ}ty)]
-                  [TCtx_hasty p (&shr{κ'}ty); TCtx_blocked p κ (&shr{κ}ty)].
+    tctx_incl E L [p ◁ &shr{κ}ty] [p ◁ &shr{κ'}ty; p ◁{κ} &shr{κ}ty].
   Proof.
     iIntros (Hκκ' tid ??) "#LFT HE HL H".
     iDestruct (elctx_interp_persist with "HE") as "#HE'".
